Monad_Play Around/Int_State_Monad_Fib.thy
@@ -1,0 +1,67 @@
+theory Int_State_Monad_Fib
+imports 
+  Main
+  "~~/src/HOL/Library/State_Monad"
+begin
+
+definition return:: "'a \<Rightarrow> ('b, 'a) state" where "return = State_Monad.return"
+definition get:: "(nat, nat) state" where "get = State (\<lambda>x. (x,x))"
+definition put:: "nat \<Rightarrow> (nat, unit) state" where "put x = State (\<lambda>_. ((),x))"
+definition skip:: "(nat, unit) state" where "skip = State (\<lambda>x. ((),x))"
+
+fun fibacc :: "nat \<Rightarrow> nat => nat \<Rightarrow> nat" where
+fa1: "fibacc 0 a b = a"| 
+fa2: "fibacc (Suc 0) a b = b"| 
+fa3: "fibacc (Suc (Suc n)) a b = fibacc (Suc n) b (a+b)"
+
+definition fib_wrap:: "nat \<Rightarrow> nat" where
+  "fib_wrap n \<equiv> fibacc n 1 1"
+
+fun monfibacc :: "nat \<Rightarrow> nat => (nat, unit) state" where
+m1:  "monfibacc 0 a = skip"| 
+m2:  "monfibacc (Suc n) a  = do{b \<leftarrow> get; put (a + b); monfibacc n b}"
+
+definition monfib_wrap where
+  "monfib_wrap n \<equiv> (monfibacc n 1)"
+
+value \<open>fibacc 9 1 1 = 55\<close>
+value \<open>snd (run_state (monfibacc 9 0) (1::nat)) = 55\<close>
+value \<open>fib_wrap 9 = 55\<close>
+value \<open>snd (run_state (monfib_wrap 9) (1::nat))\<close>
+value \<open>snd (run_state (monfib_wrap 2) (0::nat))\<close>
+value \<open>snd (run_state (monfib_wrap 0) (snd (run_state (monfib_wrap 7) 1)))\<close>
+value \<open>snd (run_state (monfib_wrap 7) 1)\<close>
+
+lemma fib_base[simp]: "snd (run_state (monfib_wrap 0) (Suc 0)) = fib_wrap 0"
+  by (simp add: fib_wrap_def monfib_wrap_def put_def skip_def)
+
+lemma fib_wrap_aux[simp]: "fib_wrap (Suc (Suc n)) = fib_wrap n + fib_wrap (Suc n)"
+  apply (induction n)
+   apply (simp add: fib_wrap_def)
+  sledgehammer
+  using Int_State_Monad.fa3 fib_wrap_def
+  sorry
+
+
+lemma monfib_aux[simp]: "snd (run_state (monfib_wrap (Suc (Suc n))) x) 
+        = snd (run_state (monfib_wrap (Suc n)) x) + snd (run_state (monfib_wrap n) x)"
+  apply (induction n arbitrary: x)
+   apply(simp_all)
+
+  sorry
+
+lemma monfib_aux[simp]: "snd (run_state (monfib_wrap (Suc (Suc n))) x) 
+        = snd (run_state (monfib_wrap (Suc n)) (snd (run_state (monfib_wrap n) x)))"
+  apply (induction n arbitrary: x)
+  sledgehammer
+   apply (simp add: put_def snd_def get_def skip_def)
+  sledgehammer
+  sorry
+
+lemma fib_basic: "snd (run_state (monfib_wrap n) 1) = fib_wrap n"
+  apply (induction n)
+   apply (simp)
+  sorry
+
+
+end
